---
documentclass: scrartcl
<!-- classoption: twocolumn -->
papersize: letter
geometry: "left=1.5cm,right=1.5cm,top=2cm,bottom=2cm"
header-includes: |
    \usepackage{mathrsfs}
---

Problem 1
============================================================

Let $Y(s) = \mathscr{L}\{y(x)\}$. Take the Laplace Transform of each side, and solve for $Y(s)$.
$$
\begin{aligned}    
    \mathscr{L}\{ y'' \}
    + \mathscr{L}\{ y \}
    &=
    \mathscr{L}\{ 2 u(x-1) \}
\\
    s^2 Y - sy(0) - y'(0)
    + Y
    &=
    \frac{ 2e^{-s} }{s}
\\
    (s^2 + 1) Y
    &=
\\
    Y
    &=
    \frac{ 2e^{-s} }{ s (s^2 + 1)}
\end{aligned}
$$

Let
${
    F = \frac{1}{s(s^2 + 1)}
}$
, and Let
${
    f = \mathscr{L}^{-1}\{F\}
}$.  
Now decompose $F$ into partial fractions.
$$
F =
\frac{A}{s}
+ \frac{Bs + C}{s^2+1}
$$
which leads to,
$$
\begin{aligned}
A(s^2+1) + (Bs+C)(s) &= 1 \\
A(s^2+1) + B(s^2) + C(s) &= 1
\end{aligned}
$$
and can be rewritten as a system of linear equations,
$$
\begin{aligned}
    A + B = 0 \\
    C = 0 \\
    A = 1 \\
\end{aligned}
$$
and solve to find $B=-1$, allowing us to rewrite $F$,
$$
F = \frac{1}{s} - \frac{s}{s+1}
$$
and we can find it's inverse laplace transform,
$$
f = 1 - \cos(x)
$$

Returning to our equation for $Y$, we can rewrite it as
$$
Y = 2 \cdot F(s) \cdot e^{-s}
$$
and find it's inverse laplace transform to be,
$$
y = 2 \cdot f(x - 1) \cdot u(x -1)
$$
plugging in our definition of $f$ we get the solution:
$$
\boxed{
y = 2 \cdot \big(1 - \cos(x-1)\big) \cdot u(x-1)
}
$$



Problem 2
============================================================

$$
\Gamma\left(\frac{11}{2} + 1\right)
\ = \
\frac{11}{2} \cdot
\Gamma\left(\frac{11}{2}\right)
\ = \
\frac{11}{2} \cdot
\Gamma\left(\frac{9}{2} + 1\right)
\ = \
\frac{9}{2} \cdot
\frac{11}{2} \cdot
\Gamma\left(\frac{9}{2}\right)
\ = \
\cdots
\ = \
\frac{11 \cdot 9 \cdot 7 \cdot 5 \cdot 3}{2^6}
\cdot
\Gamma\left(\frac{1}{2}\right)
\ = \
\frac{10395}{64} \cdot \sqrt{\pi}
$$

$$
\mathscr{L}\left\{ t^{11/2} \right\}
\ = \
\frac{
    \Gamma\left(\frac{11}{2} + 1\right)
}{
    s^{13/2}
}
\ = \
\boxed{
\frac{10395 \sqrt{\pi}}{64 \ s^{13/2}}
}
$$


Problem 3
============================================================


$$
\begin{aligned}    
    \mathscr{L}\{ y''' \}
    + 4 \mathscr{L}\{ y'' \}
    + \mathscr{L}\{ y' \}
    - 6 \mathscr{L}\{ y \}
    &=
    -12 \mathscr{L}\{ 1 \}
\\
    s^3Y - s^2y_0 - sy'_0 - y''_0
    +4 ( s^2Y - sy_0 - y'_0 )
    + (sY - y_0)
    - 6Y
    &=
    -12 /s
\\
    s^3Y - s^2 - 4s + 2
    + 4sY - 4s - 16 + sY -1 - 6Y
    &=
    -12/s
\\
    (s^3 + 4s^2 +s -6)Y
    -s^2 - 8s -15
    &=
    -12/s
\\
    (s-1)(s+2)(s+3)Y
    &=
    -12/s + s^2 + 8s + 15
\end{aligned}
$$
$$
Y
\ = \
\frac{-12 + (s^2 + 8s + 15)(s)}{
    (s)(s-1)(s+2)(s+3)
}
\ = \
\frac{s^3 + 8s^2 + 15s -12}{(s)(s-1)(s+2)(s+3)}
\ = \
\mathbf{
\frac{A}{s}
+ \frac{B}{s-1}
+ \frac{C}{s+2}
+ \frac{D}{s+3}
}
$$

$$
\mathbf{A}(s-1)(s+2)(s+3)
\ + \ \mathbf{B}(s)(s+2)(s+3)
\ + \ \mathbf{C}(s)(s-1)(s+3)
\ + \ \mathbf{D}(s)(s-1)(s+2)
\ = \ s^3 + 8s^2 + 15s -12
$$

$$
\begin{aligned}
\text{Let } s &= 0  \\
\hline
A(0-1)(0+2)(0+3) &= (0)^3 + 8(0)^2 + 15(0) - 12 \\
A(-1)(2)(3) &= -12 \\
-6 A &= -12 \\
\mathbf{A} &= \mathbf{2} \\
\end{aligned}
$$

$$
\begin{aligned}
\text{Let } s &= 1 \\
\hline
B(1)(1+2)(1+3) &= (1)^3 + 8(1)^2 + 15(1) -12 \\
B(1)(3)(4) &= 1 + 8 + 15 -12 \\
12 B &= 12 \\
\mathbf{B} &= \mathbf{1}
\end{aligned}
$$

$$
\begin{aligned}
\text{Let } s &= -2 \\
\hline
C(-2)(-2-1)(-2+3) &= (-2)^3 + 8(-2)^2 + 15(-2) -12 \\
C(-2)(-3)(1) &= -8 + 32 - 30 -12 \\
6C &= -18 \\
\mathbf{C} &= \mathbf{-3}
\end{aligned}
$$

$$
\begin{aligned}
\text{Let } s &= -3 \\
\hline
D(-3)(-3-1)(-3+2) &= (-3)^3 + 8(-3) + 15(-3) -12 \\
D(-3)(-4)(-1) &= -27 + 72 - 45 - 12 \\
\mathbf{D} &= \mathbf{1}
\end{aligned}
$$

$$
Y =
\frac{2}{s}
+ \frac{1}{s-1}
+ \frac{-3}{s+2}
+ \frac{1}{s+3}
$$

$$
\mathbf{\boxed{
y = 2 + e^{t} - 3e^{-2t} + e^{-3t}
}}
$$



Problem 4
============================================================

$$
f_3(t) =
\begin{cases}
2t+1, & 0 < t \leq 1 \\
4-t, & 1 \leq t \leq 2 \\
6-2t, & 2 \leq t\leq 3
\end{cases}
$$

$$
\begin{aligned}
f_3(t)
&= (2t+1)\Pi_{0,1}
+ (4-t)\Pi_{1,2}
+ (6-2t) \Pi_{2,3}
\end{aligned}
$$

$$
\begin{aligned}
f_3(t)
= &\enspace (2t+1)u(t-0) - (2t+1)u(t-1) \\
&+ (4-t)u(t-1) - (4-t)u(t-2) \\
&+ (6-2t)u(t-2) - (6-2t)u(t-3)
\end{aligned}
$$


$$
\begin{aligned}
F_3(t)
= &\ \quad
\mathscr{L}\{2t+1\} \\
&- \mathscr{L}\{ 2(t+1)+1 \} e^{-s} \\
&+ \mathscr{L}\{ 4-(t+1) \} e^{-s} \\
&- \mathscr{L}\{ 4-(t+2) \} e^{-2s} \\
&+ \mathscr{L}\{ 6-2(t+2) \} e^{-2s} \\
&- \mathscr{L}\{ 6-2(t+3) \} e^{-3s} \\
\end{aligned}
$$

$$
\begin{aligned}
F_3(t)
=
&\ \quad
2/s^2 + 1/s \\
&- (2/s^2 + 3/s)e^{-s} \\
&+ (-1/s^2+3/s)e^{-s} \\
&- (-1/s^2+2/s)e^{-2s} \\
&+ (-2/s^2+2/s)e^{-2s} \\
&- (-2/s^2)e^{-3s}
\end{aligned}
$$


$$
\begin{aligned}
s^2 \cdot F_3(t)
=
&\ \quad
2 + 1s \\
&- (2 + 3s)e^{-s} \\
&+ (-1+3s)e^{-s} \\
&- (-1+2s)e^{-2s} \\
&+ (-2+2s)e^{-2s} \\
&- (-2)e^{-3s}
\end{aligned}
$$

$$
\begin{aligned}
s^2 \cdot F_3(t)
=
&\ \quad
2 + 1s \\
&- 2e^{-s} - 3se^{-s} \\
&-1e^{-s} + 3se^{-s} \\
&+1e^{-2s} - 2se^{-2s} \\
&-2e^{-2s} + 2se^{-2s} \\
&+2e^{-3s}
\end{aligned}
$$


$$
s^2 \cdot F_3(t)
=
2 + 1s -3e^{-s} -1e^{-2s} +2e^{-3s}
$$

$$
F_3(t) = \frac{
    2 + s -3e^{-s} -e^{-2s} +2e^{-3s}
}{s^2}
$$

$$
F(s)
= \frac{F_T(s)}{1-e^{-sT}}
=
\boxed
{
    \frac
    {2 + s -3e^{-s} -e^{-2s} +2e^{-3s}}
    {s^2(1 - e^{-3t})}
}
$$
